Introduce `Abbreviation fset` and `Class HsOrd`. Comment out old code that will be changed.

theories/Data/FiniteMap.v
@@ -1,39 +1,448 @@
 Require Import PnV.Prelude.Prelude.
+Require Import PnV.Prelude.ConstructiveFacts.
 Require Import PnV.Prelude.X.
+Require Export PnV.Math.ThN.
+Require Export PnV.Math.OrderTheory.
+Require Export PnV.Data.HsOrd.
 Require Import PnV.Data.FiniteSet.
 
 #[local] Infix "=~=" := is_similar_to : type_scope.
+#[local] Infix "\in" := E.In.
 #[local] Infix "∈" := L.In.
 
-Module FM.
+#[local] Hint Resolve S_lt_S_intro : core.
 
-Import FS.
+Module FiniteMap.
 
 #[universes(template), projections(primitive)]
-Record alist {K : Type} {V : Type} : Type :=
-  mk_alist { kvlist : list (K * V) } as al.
-
-#[global] Arguments alist : clear implicits.
-
-#[global]
-Instance alist_isSetoid {K : Type} {V : Type} (K_hasEqDec : hasEqDec K) (V_isSetoid : isSetoid V) : isSetoid (alist K V) :=
-  { eqProp (lhs : alist K V) (rhs : alist K V) := forall k : K, eqProp (isSetoid := @option_isSetoid V V_isSetoid) (L.lookup (EQ_DEC := K_hasEqDec) k lhs.(kvlist)) (L.lookup (EQ_DEC := K_hasEqDec) k rhs.(kvlist))
-  ; eqProp_Equivalence := relation_on_image_liftsEquivalence (pi_isSetoid (fun _ => @option_isSetoid V V_isSetoid)).(eqProp_Equivalence) (fun al : alist K V => fun k : K => L.lookup (EQ_DEC := K_hasEqDec) k al.(kvlist))
+Record t {K : Type} {V : Type} {isSorted : list K -> bool} : Type :=
+  mk
+  { data : list (K * V)
+  ; data_isSorted : isSorted (map fst data) = true
   }.
 
-Definition Similarity_alist_finite_partial_map {KEY : Type} {VAL : Type} {VAL' : Type} (VAL_sim : Similarity VAL VAL') : Similarity (alist KEY VAL) (KEY -> option VAL') :=
-  fun al : alist KEY VAL => fun m' : KEY -> option VAL' => forall key, ⟪ SUBMAP1 : forall val, (key, val) ∈ al.(kvlist) -> (exists val', val =~= val' /\ m' key = Some val') ⟫ /\ ⟪ SUBMAP2 : forall val', m' key = Some val' -> (exists val, val =~= val' /\ (key, val) ∈ al.(kvlist)) ⟫.
+#[global] Arguments t : clear implicits.
+#[global] Arguments mk {K} {V} {isSorted}.
 
-#[global]
-Instance alist_corresponds_to_finite_partial_map {KEY : Type} {VAL : Type} : Similarity (alist KEY VAL) (KEY -> option VAL) :=
-  Similarity_alist_finite_partial_map eq.
-
-Theorem alist_corresponds_to_finite_partial_map_iff (KEY : Type) (VAL : Type) (al : alist KEY VAL) (m : KEY -> option VAL)
-  : al =~= m <-> (forall k, forall v, (k, v) ∈ al.(kvlist) <-> m k = Some v).
+Lemma t_eq_iff {K : Type} {V : Type} {isSorted : list K -> bool} (m : FiniteMap.t K V isSorted) (m' : FiniteMap.t K V isSorted)
+  : m = m' <-> m.(data) = m'.(data).
 Proof.
-  done!.
+  split.
+  - intros H_eq. subst m'. reflexivity.
+  - revert m m'.
+    assert (claim : forall data1 : list (K * V), forall data2 : list (K * V), forall data1_isSorted : isSorted (map fst data1) = true, forall data2_isSorted : isSorted (map fst data2) = true, data1 = data2 -> {| data := data1; data_isSorted := data1_isSorted |} = {| data := data2; data_isSorted := data2_isSorted |}).
+    { ii. subst data2. enough (HH : data1_isSorted = data2_isSorted) by now rewrite HH. eapply eq_pirrel_fromEqDec. }
+    intros X X' H_eq. exact (claim X.(data) X'.(data) X.(data_isSorted) X'.(data_isSorted) H_eq).
 Qed.
 
-#[global] Hint Rewrite alist_corresponds_to_finite_partial_map_iff : simplication_hints.
+End FiniteMap.
 
-End FM.
+Abbreviation finite_map K V := (FiniteMap.t K V (isSorted compare)).
+
+Section BASICS.
+
+Context {K : Type} {V : Type} {POSET_K : isPoset K} {HsOrd_K : HsOrd K (POSET := POSET_K)}.
+
+Definition lookup' (k0 : K) : list (K * V) -> option V :=
+  fix go (kvs : list (K * V)) {struct kvs} : option V :=
+  match kvs with
+  | [] => None
+  | (k, v) :: kvs =>
+    match compare k0 k with
+    | Lt => None
+    | Eq => Some v
+    | Gt => go kvs
+    end
+  end.
+
+Definition lookup (k : K) (m : finite_map K V) : option V :=
+  lookup' k m.(FiniteMap.data).
+
+Lemma lookup'_nil (k0 : K)
+  : lookup' k0 [] = None.
+Proof.
+  reflexivity.
+Qed.
+
+Lemma lookup'_cons (k0 : K) (k : K) (v : V) (kvs : list (K * V)) :
+  lookup' k0 ((k, v) :: kvs) =
+  match compare k0 k with
+  | Lt => None
+  | Eq => Some v
+  | Gt => lookup' k0 kvs
+  end.
+Proof.
+  reflexivity.
+Qed.
+
+Lemma lookup'_lt_None (k0 : K) (kvs : list (K * V))
+  (LT : forall q : K * V, q ∈ kvs -> compare k0 (fst q) = Lt)
+  : lookup' k0 kvs = None.
+Proof.
+  destruct kvs as [ | [k1 v1] kvs]; trivial.
+  pose proof (LT (k1, v1) (or_introl eq_refl)) as LT1. simpl in LT1.
+  rewrite lookup'_cons, LT1. reflexivity.
+Qed.
+
+Lemma isSorted_map_fst_cons_iff (p : K * V) (ps : list (K * V))
+  : isSorted compare (map fst (p :: ps)) = true <-> ((forall q : K * V, q ∈ ps -> compare (fst p) (fst q) = Lt) /\ isSorted compare (map fst ps) = true).
+Proof.
+  cbn [map]. rewrite isSorted_cons_iff. split.
+  - intros [SORTED_hd SORTED_tl]. split; trivial.
+    intros q q_in. eapply SORTED_hd. eapply L.in_map. exact q_in.
+  - intros [SORTED_hd SORTED_tl]. split; trivial.
+    intros z z_in. rewrite L.in_map_iff in z_in.
+    destruct z_in as (q & fst_q_eq_z & q_in). subst z. exact (SORTED_hd q q_in).
+Qed.
+
+Theorem finite_map_eq_spec (m : finite_map K V) (m' : finite_map K V)
+  : m = m' <-> (forall k, lookup k m = lookup k m').
+Proof.
+  rewrite FiniteMap.t_eq_iff. unfold lookup. split.
+  - intros H_eq k. rewrite H_eq. reflexivity.
+  - intros EXT.
+    pose proof (fun p : K * V => fun ps : list (K * V) => proj1 (isSorted_map_fst_cons_iff p ps)) as HD_TL.
+    pose proof lookup'_lt_None as LT_None.
+    pose proof (m.(FiniteMap.data_isSorted)) as kvs_isSorted.
+    pose proof (m'.(FiniteMap.data_isSorted)) as kvs'_isSorted.
+    set (kvs := m.(FiniteMap.data)) in *. set (kvs' := m'.(FiniteMap.data)) in *.
+    clearbody kvs kvs'. clear m m'. revert kvs_isSorted kvs' kvs'_isSorted EXT.
+    induction kvs as [ | [k v] kvs IH]; intros kvs_isSorted [ | [k' v'] kvs'] kvs'_isSorted EXT.
+    + reflexivity.
+    + pose proof (EXT k') as H. cbn [lookup'] in H. rewrite compare_refl in H. discriminate H.
+    + pose proof (EXT k) as H. cbn [lookup'] in H. rewrite compare_refl in H. discriminate H.
+    + pose proof (HD_TL (k, v) kvs kvs_isSorted) as [k_lt_kvs kvs_isSorted'].
+      pose proof (HD_TL (k', v') kvs' kvs'_isSorted) as [k'_lt_kvs' kvs'_isSorted'].
+      simpl in k_lt_kvs, k'_lt_kvs'.
+      assert (k_eq_k' : k = k').
+      { destruct (compare k k') as [ | | ] eqn: H_OBS.
+        - exact (proj1 (compare_eq_iff k k') H_OBS).
+        - exfalso. pose proof (EXT k) as H. cbn [lookup'] in H.
+          rewrite compare_refl, H_OBS in H. discriminate H.
+        - exfalso. pose proof (EXT k') as H. cbn [lookup'] in H.
+          rewrite compare_refl, (compare_Gt_flip k k' H_OBS) in H. discriminate H.
+      }
+      subst k'.
+      assert (v_eq_v' : v = v').
+      { pose proof (EXT k) as H. cbn [lookup'] in H. rewrite compare_refl in H. now inversion H. }
+      subst v'. f_equal. eapply IH; trivial. intros k0.
+      destruct (compare k0 k) as [ | | ] eqn: H_OBS.
+      * rewrite compare_eq_iff in H_OBS. subst k0.
+        rewrite (LT_None k kvs k_lt_kvs), (LT_None k kvs' k'_lt_kvs'). reflexivity.
+      * assert (H1 : lookup' k0 kvs = None).
+        { eapply LT_None. intros q q_in. exact (compare_Lt_trans k0 k (fst q) H_OBS (k_lt_kvs q q_in)). }
+        assert (H2 : lookup' k0 kvs' = None).
+        { eapply LT_None. intros q q_in. exact (compare_Lt_trans k0 k (fst q) H_OBS (k'_lt_kvs' q q_in)). }
+        rewrite H1, H2. reflexivity.
+      * pose proof (EXT k0) as H. cbn [lookup'] in H. rewrite H_OBS in H. exact H.
+Qed.
+
+Lemma lookup'_spec (kvs : list (K * V))
+  (kvs_isSorted : isSorted compare (map fst kvs) = true)
+  : forall k : K, forall v : V, lookup' k kvs = Some v <-> (k, v) ∈ kvs.
+Proof.
+  revert kvs_isSorted. induction kvs as [ | [k1 v1] kvs IH]; intros kvs_isSorted k v.
+  - rewrite lookup'_nil. simpl. split; [intros H_eq; discriminate H_eq | tauto].
+  - rewrite isSorted_map_fst_cons_iff in kvs_isSorted.
+    destruct kvs_isSorted as [k1_lt_kvs kvs_isSorted]. simpl in k1_lt_kvs.
+    pose proof (IH kvs_isSorted k v) as IH'. rewrite lookup'_cons. simpl.
+    destruct (compare k k1) as [ | | ] eqn: H_OBS.
+    + rewrite compare_eq_iff in H_OBS. subst k1. split.
+      * intros H_eq. left. congruence.
+      * intros [H_eq | H_in]; [congruence | ].
+        exfalso. pose proof (k1_lt_kvs (k, v) H_in) as LT. simpl in LT.
+        rewrite compare_refl in LT. discriminate LT.
+    + split; [intros H_eq; discriminate H_eq | ]. intros [H_eq | H_in].
+      * exfalso. inversion H_eq; subst k1 v1. rewrite compare_refl in H_OBS. discriminate H_OBS.
+      * exfalso. pose proof (k1_lt_kvs (k, v) H_in) as LT. simpl in LT.
+        pose proof (compare_Lt_trans k k1 k H_OBS LT) as LT'.
+        rewrite compare_refl in LT'. discriminate LT'.
+    + rewrite IH'. split; [intros H_in; right; exact H_in | ].
+      intros [H_eq | H_in]; trivial.
+      exfalso. inversion H_eq; subst k1 v1. rewrite compare_refl in H_OBS. discriminate H_OBS.
+Qed.
+
+Theorem lookup_spec (m : finite_map K V) (k : K) (v : V)
+  : lookup k m = Some v <-> (k, v) ∈ m.(FiniteMap.data).
+Proof.
+  exact (lookup'_spec m.(FiniteMap.data) m.(FiniteMap.data_isSorted) k v).
+Qed.
+
+Definition empty : finite_map K V :=
+  FiniteMap.mk [] eq_refl.
+
+Theorem lookup_empty (k : K)
+  : lookup k empty = None.
+Proof.
+  reflexivity.
+Qed.
+
+Definition insert' (k0 : K) (v0 : V) : list (K * V) -> list (K * V) :=
+  fix go (kvs : list (K * V)) {struct kvs} : list (K * V) :=
+  match kvs with
+  | [] => [(k0, v0)]
+  | (k, v) :: kvs =>
+    match compare k0 k with
+    | Lt => (k0, v0) :: (k, v) :: kvs
+    | Eq => (k0, v0) :: kvs
+    | Gt => (k, v) :: go kvs
+    end
+  end.
+
+Lemma insert'_nil (k0 : K) (v0 : V)
+  : insert' k0 v0 [] = [(k0, v0)].
+Proof.
+  reflexivity.
+Qed.
+
+Lemma insert'_cons (k0 : K) (v0 : V) (k : K) (v : V) (kvs : list (K * V)) :
+  insert' k0 v0 ((k, v) :: kvs) =
+  match compare k0 k with
+  | Lt => (k0, v0) :: (k, v) :: kvs
+  | Eq => (k0, v0) :: kvs
+  | Gt => (k, v) :: insert' k0 v0 kvs
+  end.
+Proof.
+  reflexivity.
+Qed.
+
+Lemma map_fst_insert' (k0 : K) (v0 : V) (kvs : list (K * V))
+  : map fst (insert' k0 v0 kvs) = FS.insert k0 (map fst kvs).
+Proof.
+  induction kvs as [ | [k v] kvs IH]; trivial.
+  rewrite insert'_cons.
+  change (FS.insert k0 (map fst ((k, v) :: kvs)))
+    with (match compare k0 k with Lt => k0 :: k :: map fst kvs | Eq => k :: map fst kvs | Gt => k :: FS.insert k0 (map fst kvs) end).
+  destruct (compare k0 k) as [ | | ] eqn: H_OBS.
+  - cbn [map fst]. f_equal. exact (proj1 (compare_eq_iff k0 k) H_OBS).
+  - reflexivity.
+  - cbn [map fst]. f_equal. exact IH.
+Qed.
+
+Lemma isSorted_insert' (k0 : K) (v0 : V) (kvs : list (K * V))
+  (kvs_isSorted : isSorted compare (map fst kvs) = true)
+  : isSorted compare (map fst (insert' k0 v0 kvs)) = true.
+Proof.
+  rewrite map_fst_insert'. exact (FS.isSorted_insert k0 (map fst kvs) kvs_isSorted).
+Qed.
+
+Definition insert (k : K) (v : V) (m : finite_map K V) : finite_map K V :=
+  FiniteMap.mk (insert' k v m.(FiniteMap.data)) (isSorted_insert' k v m.(FiniteMap.data) m.(FiniteMap.data_isSorted)).
+
+Theorem lookup_insert_eq (k : K) (v : V) (m : finite_map K V)
+  : lookup k (insert k v m) = Some v.
+Proof.
+  unfold lookup, insert. cbn [FiniteMap.data].
+  generalize m.(FiniteMap.data) as kvs. clear m.
+  induction kvs as [ | [k1 v1] kvs IH].
+  - rewrite insert'_nil, lookup'_cons, compare_refl. reflexivity.
+  - rewrite insert'_cons. destruct (compare k k1) as [ | | ] eqn: H_OBS.
+    + rewrite lookup'_cons, compare_refl. reflexivity.
+    + rewrite lookup'_cons, compare_refl. reflexivity.
+    + rewrite lookup'_cons, H_OBS. exact IH.
+Qed.
+
+Theorem lookup_insert_ne (k : K) (v : V) (m : finite_map K V) (k0 : K)
+  (NE : k0 ≠ k)
+  : lookup k0 (insert k v m) = lookup k0 m.
+Proof.
+  unfold lookup, insert. cbn [FiniteMap.data].
+  generalize m.(FiniteMap.data) as kvs. clear m.
+  induction kvs as [ | [k1 v1] kvs IH].
+  - rewrite insert'_nil, !lookup'_cons, lookup'_nil.
+    destruct (compare k0 k) as [ | | ] eqn: H_OBS; trivial.
+    exfalso. rewrite compare_eq_iff in H_OBS. contradiction.
+  - rewrite insert'_cons. destruct (compare k k1) as [ | | ] eqn: H_OBS1.
+    + rewrite compare_eq_iff in H_OBS1. subst k1. rewrite !lookup'_cons.
+      destruct (compare k0 k) as [ | | ] eqn: H_OBS2; trivial.
+      exfalso. rewrite compare_eq_iff in H_OBS2. contradiction.
+    + rewrite lookup'_cons. destruct (compare k0 k) as [ | | ] eqn: H_OBS2.
+      * exfalso. rewrite compare_eq_iff in H_OBS2. contradiction.
+      * rewrite lookup'_cons, (compare_Lt_trans k0 k k1 H_OBS2 H_OBS1). reflexivity.
+      * reflexivity.
+    + rewrite !lookup'_cons. destruct (compare k0 k1) as [ | | ]; trivial.
+Qed.
+
+Definition remove' (k0 : K) : list (K * V) -> list (K * V) :=
+  fix go (kvs : list (K * V)) {struct kvs} : list (K * V) :=
+  match kvs with
+  | [] => []
+  | (k, v) :: kvs =>
+    match compare k0 k with
+    | Lt => (k, v) :: kvs
+    | Eq => kvs
+    | Gt => (k, v) :: go kvs
+    end
+  end.
+
+Lemma remove'_nil (k0 : K)
+  : remove' k0 [] = [].
+Proof.
+  reflexivity.
+Qed.
+
+Lemma remove'_cons (k0 : K) (k : K) (v : V) (kvs : list (K * V)) :
+  remove' k0 ((k, v) :: kvs) =
+  match compare k0 k with
+  | Lt => (k, v) :: kvs
+  | Eq => kvs
+  | Gt => (k, v) :: remove' k0 kvs
+  end.
+Proof.
+  reflexivity.
+Qed.
+
+Lemma in_remove'_incl (k0 : K) (kvs : list (K * V))
+  : forall q : K * V, q ∈ remove' k0 kvs -> q ∈ kvs.
+Proof.
+  induction kvs as [ | [k v] kvs IH]; trivial.
+  intros q. rewrite remove'_cons. destruct (compare k0 k) as [ | | ].
+  - intros H_in. right. exact H_in.
+  - intros H_in. exact H_in.
+  - intros [H_eq | H_in]; [left; exact H_eq | right; exact (IH q H_in)].
+Qed.
+
+Lemma isSorted_remove' (k0 : K) (kvs : list (K * V))
+  (kvs_isSorted : isSorted compare (map fst kvs) = true)
+  : isSorted compare (map fst (remove' k0 kvs)) = true.
+Proof.
+  revert kvs_isSorted. induction kvs as [ | [k v] kvs IH]; intros kvs_isSorted; trivial.
+  pose proof (proj1 (isSorted_map_fst_cons_iff (k, v) kvs) kvs_isSorted) as [k_lt_kvs kvs_isSorted'].
+  simpl in k_lt_kvs. rewrite remove'_cons. destruct (compare k0 k) as [ | | ].
+  - exact kvs_isSorted'.
+  - exact kvs_isSorted.
+  - rewrite isSorted_map_fst_cons_iff. simpl. split; [ | exact (IH kvs_isSorted')].
+    intros q q_in. exact (k_lt_kvs q (in_remove'_incl k0 kvs q q_in)).
+Qed.
+
+Definition remove (k : K) (m : finite_map K V) : finite_map K V :=
+  FiniteMap.mk (remove' k m.(FiniteMap.data)) (isSorted_remove' k m.(FiniteMap.data) m.(FiniteMap.data_isSorted)).
+
+Theorem lookup_remove_eq (k : K) (m : finite_map K V)
+  : lookup k (remove k m) = None.
+Proof.
+  unfold lookup, remove. cbn [FiniteMap.data].
+  pose proof (m.(FiniteMap.data_isSorted)) as kvs_isSorted.
+  generalize dependent m.(FiniteMap.data). intros kvs. clear m.
+  induction kvs as [ | [k1 v1] kvs IH]; intros kvs_isSorted; trivial.
+  pose proof (proj1 (isSorted_map_fst_cons_iff (k1, v1) kvs) kvs_isSorted) as [k1_lt_kvs kvs_isSorted'].
+  simpl in k1_lt_kvs. rewrite remove'_cons. destruct (compare k k1) as [ | | ] eqn: H_OBS.
+  - eapply lookup'_lt_None. intros q q_in.
+    rewrite compare_eq_iff in H_OBS. subst k1. exact (k1_lt_kvs q q_in).
+  - rewrite lookup'_cons, H_OBS. reflexivity.
+  - rewrite lookup'_cons, H_OBS. exact (IH kvs_isSorted').
+Qed.
+
+Theorem lookup_remove_ne (k : K) (m : finite_map K V) (k0 : K)
+  (NE : k0 ≠ k)
+  : lookup k0 (remove k m) = lookup k0 m.
+Proof.
+  unfold lookup, remove. cbn [FiniteMap.data].
+  pose proof (m.(FiniteMap.data_isSorted)) as kvs_isSorted.
+  generalize dependent m.(FiniteMap.data). intros kvs. clear m.
+  induction kvs as [ | [k1 v1] kvs IH]; intros kvs_isSorted; trivial.
+  pose proof (proj1 (isSorted_map_fst_cons_iff (k1, v1) kvs) kvs_isSorted) as [k1_lt_kvs kvs_isSorted'].
+  simpl in k1_lt_kvs. rewrite remove'_cons. destruct (compare k k1) as [ | | ] eqn: H_OBS1.
+  - rewrite compare_eq_iff in H_OBS1. subst k1.
+    rewrite lookup'_cons. destruct (compare k0 k) as [ | | ] eqn: H_OBS2.
+    + exfalso. rewrite compare_eq_iff in H_OBS2. contradiction.
+    + eapply lookup'_lt_None. intros q q_in.
+      exact (compare_Lt_trans k0 k (fst q) H_OBS2 (k1_lt_kvs q q_in)).
+    + reflexivity.
+  - reflexivity.
+  - rewrite !lookup'_cons. destruct (compare k0 k1) as [ | | ]; trivial.
+    exact (IH kvs_isSorted').
+Qed.
+
+Definition keys (m : finite_map K V) : fset K :=
+  FSet.mk (map fst m.(FiniteMap.data)) m.(FiniteMap.data_isSorted).
+
+Theorem in_keys_iff (m : finite_map K V) (k : K)
+  : k ∈ (keys m).(FSet.data) <-> (exists v : V, lookup k m = Some v).
+Proof.
+  cbv [keys]; simpl. rewrite L.in_map_iff. split.
+  - intros ([k1 v1] & fst_eq & p_in). simpl in fst_eq. subst k1.
+    exists v1. rewrite lookup_spec. exact p_in.
+  - intros [v H_eq]. rewrite lookup_spec in H_eq. exists (k, v). split; auto.
+Qed.
+
+End BASICS.
+
+Section SIMILARITY.
+
+#[local] Existing Instance Similarity_option_option.
+
+Definition Similarity_finite_map_partial_map {K : Type} {V : Type} {POSET_K : isPoset K} {HsOrd_K : HsOrd K (POSET := POSET_K)} {K' : Type} {V' : Type} (Similarity_K_K' : Similarity K K') (Similarity_V_V' : Similarity V V') : Similarity (finite_map K V) (K' -> option V') :=
+  fun m : finite_map K V => fun m' : K' -> option V' => forall k : K, forall k' : K', k =~= k' -> lookup k m =~= m' k'.
+
+Context {K : Type} {V : Type} {POSET_K : isPoset K} {HsOrd_K : HsOrd K (POSET := POSET_K)}.
+
+#[global]
+Instance finite_map_corresponds_to_partial_map : Similarity (finite_map K V) (K -> option V) :=
+  Similarity_finite_map_partial_map eq eq.
+
+Theorem finite_map_corresponds_to_partial_map_iff (m : finite_map K V) (m' : K -> option V)
+  : m =~= m' <-> (forall x : K, lookup x m = m' x).
+Proof.
+  split.
+  - intros H_sim. do 4 red in H_sim. intros x. pose proof (H_sim x x eq_refl) as H. destruct H; f_equal; auto.
+  - intros H_eq. do 4 red. intros x x' x_eq_x'. change (x = x') in x_eq_x'. subst x'.
+    pose proof (H_eq x) as H. destruct (lookup x m), (m' x); try congruence; econs; red; congruence.
+Qed.
+
+End SIMILARITY.
+
+Section HsOrd_finite_map.
+
+#[local] Obligation Tactic := idtac.
+
+Context {K : Type} {V : Type} {POSET_K : isPoset K} {HsOrd_K : HsOrd K (POSET := POSET_K)} {POSET_V : isPoset V} {HsOrd_V : HsOrd V (POSET := POSET_V)}.
+
+#[local, program]
+Instance finite_map_isProset : isProset (finite_map K V) :=
+  { leProp (m : finite_map K V) (m' : finite_map K V) := m.(FiniteMap.data) =< m'.(FiniteMap.data)
+  ; Proset_isSetoid := mkSetoid_from_eq
+  }.
+Next Obligation.
+  split.
+  - intros m. reflexivity.
+  - intros m m' m'' m_le_m' m'_le_m''. now transitivity m'.(FiniteMap.data).
+Qed.
+Next Obligation.
+  intros m m'. unfold flip. split.
+  - intros m_eq_m'. change (m = m') in m_eq_m'. subst m'. split; reflexivity.
+  - intros [m_le_m' m'_le_m]. change (m = m'). rewrite FiniteMap.t_eq_iff. rewrite <- Poset_eqProp_spec.
+    exact (leProp_antisymmetry m.(FiniteMap.data) m'.(FiniteMap.data) m_le_m' m'_le_m).
+Qed.
+
+#[global]
+Instance finite_map_isPoset : isPoset (finite_map K V) :=
+  { Poset_isProset := finite_map_isProset
+  ; Poset_eqProp_spec (m : finite_map K V) (m' : finite_map K V) := conj (fun H : m = m' => H) (fun H : m = m' => H)
+  }.
+
+#[local, program]
+Instance finite_map_hsOrd : hsOrd (finite_map K V) (PROSET := Poset_isProset) :=
+  { compare (m : finite_map K V) (m' : finite_map K V) := compare m.(FiniteMap.data) m'.(FiniteMap.data) }.
+Next Obligation.
+  intros m m' OBS_Lt. pose proof (compare_Lt m.(FiniteMap.data) m'.(FiniteMap.data) OBS_Lt) as [LE NE]. split.
+  - exact LE.
+  - intros m_eq_m'. contradiction NE. do 6 red in m_eq_m' |- *.
+    rewrite -> FiniteMap.t_eq_iff in m_eq_m'. rewrite m_eq_m'. reflexivity.
+Qed.
+Next Obligation.
+  intros m m' OBS_Eq. pose proof (compare_Eq m.(FiniteMap.data) m'.(FiniteMap.data) OBS_Eq) as H_eq.
+  rewrite Poset_eqProp_spec in H_eq. exact (proj2 (FiniteMap.t_eq_iff m m') H_eq).
+Qed.
+Next Obligation.
+  intros m m' OBS_Gt. pose proof (compare_Gt m.(FiniteMap.data) m'.(FiniteMap.data) OBS_Gt) as [LE NE]. split.
+  - exact LE.
+  - intros m_eq_m'. contradiction NE. do 6 red in m_eq_m' |- *.
+    rewrite -> FiniteMap.t_eq_iff in m_eq_m'. rewrite m_eq_m'. reflexivity.
+Qed.
+
+#[global]
+Instance HsOrd_finite_map : HsOrd (finite_map K V) (POSET := finite_map_isPoset) :=
+  { HsOrd_hsOrd := finite_map_hsOrd }.
+
+End HsOrd_finite_map.
