theories/Data/FiniteSet.v
@@ -1,6 +1,9 @@
 Require Import PnV.Prelude.Prelude.
+Require Import PnV.Prelude.ConstructiveFacts.
 Require Import PnV.Prelude.X.
 Require Export PnV.Math.ThN.
+Require Export PnV.Math.OrderTheory.
+Require Export PnV.Data.HsOrd.
 
 #[local] Infix "=~=" := is_similar_to : type_scope.
 #[local] Infix "\in" := E.In.
@@ -8,281 +11,537 @@ Require Export PnV.Math.ThN.
 
 #[local] Hint Resolve S_lt_S_intro : core.
 
-Universe U_fs.
+Module FSet.
 
-Constraint U_fs <= U_discourse.
+#[universes(template), projections(primitive)]
+Record t {A : Type} {isSorted : list A -> bool} : Type :=
+  mk
+  { data : list A
+  ; data_isSorted : isSorted data = true
+  }.
+
+#[global] Arguments t : clear implicits.
+#[global] Arguments mk {A} {isSorted}.
+
+Lemma t_eq_iff {A : Type} {isSorted : list A -> bool} (X : FSet.t A isSorted) (X' : FSet.t A isSorted)
+  : X = X' <-> X.(data) = X'.(data).
+Proof.
+  split.
+  - intros H_eq. subst X'. reflexivity.
+  - revert X X'.
+    assert (claim : forall data1 : list A, forall data2 : list A, forall data1_isSorted : isSorted data1 = true, forall data2_isSorted : isSorted data2 = true, data1 = data2 -> {| data := data1; data_isSorted := data1_isSorted |} = {| data := data2; data_isSorted := data2_isSorted |}).
+    { ii. subst data2. enough (HH : data1_isSorted = data2_isSorted) by now rewrite HH. eapply eq_pirrel_fromEqDec. }
+    intros X X' H_eq. exact (claim X.(data) X'.(data) X.(data_isSorted) X'.(data_isSorted) H_eq).
+Qed.
+
+End FSet.
+
+Abbreviation fset A := (FSet.t A (isSorted compare)).
+
+Theorem fset_eq_spec (A : Type) (POSET : isPoset A) (HS_ORD : HsOrd A (POSET := POSET)) (X : fset A) (X' : fset A)
+  : X = X' <-> (forall z : A, L.In z X.(FSet.data) <-> L.In z X'.(FSet.data)).
+Proof.
+  rewrite FSet.t_eq_iff. split.
+  - ii. rewrite H. reflexivity.
+  - intros EXT.
+    assert (LT_asym : forall x1 : A, forall x2 : A, compare x1 x2 = Lt -> compare x2 x1 = Lt -> False).
+    { intros x1 x2 LT1 LT2.
+      pose proof (compare_Lt x1 x2 LT1) as [x1_le_x2 x1_ne_x2].
+      pose proof (compare_Lt x2 x1 LT2) as [x2_le_x1 _].
+      contradiction x1_ne_x2. eapply leProp_antisymmetry; assumption.
+    }
+    assert (LT_neq : forall x1 : A, forall x2 : A, compare x1 x2 = Lt -> x1 <> x2).
+    { intros x1 x2 LT x1_eq_x2. subst x2.
+      pose proof (compare_Lt x1 x1 LT) as [_ x1_ne_x1].
+      contradiction x1_ne_x1. reflexivity.
+    }
+    assert (HD_TL : forall x : A, forall zs : list A, isSorted compare (x :: zs) = true -> ((forall z : A, z ∈ zs -> compare x z = Lt) /\ isSorted compare zs = true)).
+    { intros x zs SORTED. simpl in SORTED. rewrite andb_true_iff in SORTED.
+      destruct SORTED as [SORTED_hd SORTED_tl]. rewrite forallb_forall in SORTED_hd.
+      split; trivial. intros z z_in. rewrite <- eqb_eq. exact (SORTED_hd z z_in).
+    }
+    pose proof (X.(FSet.data_isSorted)) as xs_isSorted.
+    pose proof (X'.(FSet.data_isSorted)) as ys_isSorted.
+    set (xs := X.(FSet.data)) in *. set (ys := X'.(FSet.data)) in *.
+    clearbody xs ys. clear X X'. revert xs_isSorted ys ys_isSorted EXT.
+    induction xs as [ | x xs IH]; intros xs_isSorted [ | y ys] ys_isSorted EXT.
+    + reflexivity.
+    + exfalso. exact (proj2 (EXT y) (or_introl eq_refl)).
+    + exfalso. exact (proj1 (EXT x) (or_introl eq_refl)).
+    + pose proof (HD_TL x xs xs_isSorted) as [x_lt_xs xs_isSorted'].
+      pose proof (HD_TL y ys ys_isSorted) as [y_lt_ys ys_isSorted'].
+      assert (x_eq_y : x = y).
+      { pose proof (proj1 (EXT x) (or_introl eq_refl)) as [y_eq_x | x_in_ys].
+        - symmetry. exact y_eq_x.
+        - pose proof (proj2 (EXT y) (or_introl eq_refl)) as [x_eq_y | y_in_xs].
+          + exact x_eq_y.
+          + exfalso. exact (LT_asym x y (x_lt_xs y y_in_xs) (y_lt_ys x x_in_ys)).
+      }
+      subst y. f_equal. eapply IH; trivial. intros z. split.
+      * intros z_in_xs. pose proof (proj1 (EXT z) (or_intror z_in_xs)) as [x_eq_z | z_in_ys].
+        { exfalso. exact (LT_neq x z (x_lt_xs z z_in_xs) x_eq_z). }
+        { exact z_in_ys. }
+      * intros z_in_ys. pose proof (proj2 (EXT z) (or_intror z_in_ys)) as [x_eq_z | z_in_xs].
+        { exfalso. exact (LT_neq x z (y_lt_ys z z_in_ys) x_eq_z). }
+        { exact z_in_xs. }
+Qed.
+
+Section HsOrd_fset.
+
+#[local] Obligation Tactic := idtac.
+
+Context {A : Type} {POSET : isPoset A} {HS_ORD : HsOrd A (POSET := POSET)}.
+
+#[local, program]
+Instance fset_isProset : isProset (fset A) :=
+  { leProp (X : fset A) (X' : fset A) := X.(FSet.data) =< X'.(FSet.data)
+  ; Proset_isSetoid := mkSetoid_from_eq
+  }.
+Next Obligation.
+  split.
+  - intros X. reflexivity.
+  - intros X X' X'' X_le_X' X'_le_X''. transitivity X'.(FSet.data); assumption.
+Qed.
+Next Obligation.
+  intros X X'. unfold flip. split.
+  - intros X_eq_X'. change (X = X') in X_eq_X'. subst X'. split; reflexivity.
+  - intros [X_le_X' X'_le_X]. change (X = X'). rewrite FSet.t_eq_iff. rewrite <- Poset_eqProp_spec.
+    exact (leProp_antisymmetry X.(FSet.data) X'.(FSet.data) X_le_X' X'_le_X).
+Qed.
+
+#[global]
+Instance fset_isPoset : isPoset (fset A) :=
+  { Poset_isProset := fset_isProset
+  ; Poset_eqProp_spec (X : fset A) (X' : fset A) := conj (fun H : X = X' => H) (fun H : X = X' => H)
+  }.
+
+#[local, program]
+Instance fset_hsOrd : hsOrd (fset A) (PROSET := Poset_isProset) :=
+  { compare (X : fset A) (X' : fset A) := compare X.(FSet.data) X'.(FSet.data) }.
+Next Obligation.
+  intros X X' OBS_Lt. pose proof (compare_Lt X.(FSet.data) X'.(FSet.data) OBS_Lt) as [LE NE]. split.
+  - exact LE.
+  - intros X_eq_X'. contradiction NE. do 6 red in X_eq_X' |- *. subst X'. reflexivity.
+Qed.
+Next Obligation.
+  intros X X' OBS_Eq. pose proof (compare_Eq X.(FSet.data) X'.(FSet.data) OBS_Eq) as H_eq.
+  rewrite Poset_eqProp_spec in H_eq. exact (proj2 (FSet.t_eq_iff X X') H_eq).
+Qed.
+Next Obligation.
+  intros X X' OBS_Gt. pose proof (compare_Gt X.(FSet.data) X'.(FSet.data) OBS_Gt) as [LE NE]. split.
+  - exact LE.
+  - intros X_eq_X'. contradiction NE. do 6 red in X_eq_X' |- *. subst X'. reflexivity.
+Qed.
+
+#[global]
+Instance HsOrd_fset : HsOrd (fset A) (POSET := fset_isPoset) :=
+  { HsOrd_hsOrd := fset_hsOrd }.
+
+End HsOrd_fset.
 
 Module FS.
 
-#[universes(polymorphic=yes)]
-Definition fin_ensemble@{u | } (Elem : Type@{u}) : Type@{u} :=
-  list Elem.
+Section SIMILARITY.
 
-Definition Similarity_list_finite_ensemble {ELEM : Type} {ELEM' : Type} (ELEM_sim : Similarity ELEM ELEM') : Similarity (fin_ensemble ELEM) (ensemble ELEM') :=
-  fun xs : fin_ensemble ELEM => fun X' : ensemble ELEM' => forall x : ELEM, forall x' : ELEM', x =~= x' -> ⟪ IFF : x ∈ xs <-> x' \in X' ⟫.
+Definition Similarity_fset_ensemble {A : Type} {A' : Type} {POSET : isPoset A} {HS_ORD : HsOrd A (POSET := POSET)} (Sim_A_A' : Similarity A A') : Similarity (fset A) (ensemble A') :=
+  fun X : fset A => fun X' : ensemble A' => forall x : A, forall x' : A', x =~= x' -> (x ∈ X.(FSet.data) <-> x' \in X').
 
-#[global]
-Instance list_corresponds_to_finite_ensemble {ELEM : Type} : Similarity (fin_ensemble ELEM) (ensemble ELEM) :=
-  Similarity_list_finite_ensemble eq.
-
-Theorem list_corresponds_to_finite_ensemble_iff (A : Type) (xs : fin_ensemble A) (X : ensemble A)
-  : xs =~= X <-> (forall x, x ∈ xs <-> x \in X).
-Proof.
-  done!.
-Qed.
-
-#[global] Hint Rewrite list_corresponds_to_finite_ensemble_iff : simplication_hints.
-
-Theorem list_corresponds_to_finite_ensemble_flat_map {A : Type} {B : Type} (xs : fin_ensemble A) (X : ensemble A) (f : A -> fin_ensemble B) (F : A -> ensemble B)
-  (xs_sim : xs =~= X)
-  (f_sim : forall x, x ∈ xs -> f x =~= F x)
-  : L.flat_map f xs =~= (X >>= F).
-Proof.
-  rewrite list_corresponds_to_finite_ensemble_iff.
-  intros b. rewrite L.in_flat_map. split.
-  - intros (x & x_in & b_in). exists x. split.
-    + rewrite list_corresponds_to_finite_ensemble_iff in xs_sim.
-      now rewrite <- xs_sim.
-    + find fx_sim by f_sim.
-      rewrite list_corresponds_to_finite_ensemble_iff in fx_sim.
-      now rewrite <- fx_sim.
-  - intros (x & x_in & b_in). exists x. split.
-    + rewrite list_corresponds_to_finite_ensemble_iff in xs_sim.
-      now rewrite -> xs_sim.
-    + rewrite list_corresponds_to_finite_ensemble_iff in xs_sim.
-      rewrite <- xs_sim in x_in. find fx_sim by f_sim.
-      rewrite list_corresponds_to_finite_ensemble_iff in fx_sim.
-      now rewrite -> fx_sim.
-Qed.
-
-#[global] Typeclasses Opaque fin_ensemble.
-
-#[global] Hint Rewrite L.in_concat : simplication_hints.
-#[global] Hint Rewrite L.in_map_iff : simplication_hints.
-#[global] Hint Rewrite L.in_flat_map : simplication_hints.
-#[global] Hint Rewrite length_app : simplication_hints.
-#[global] Hint Rewrite length_map : simplication_hints.
-
-#[global, program]
-Instance fin_ensemble_isSetoid (Elem : Type@{U_fs}) (Elem_isSetoid : isSetoid Elem) : isSetoid (fin_ensemble@{U_fs} Elem) :=
-  { eqProp (lhs : list Elem) (rhs : list Elem) := (forall e : Elem, forall IN : e ∈ lhs, exists e', e' ∈ rhs /\ e == e') /\ (forall e : Elem, forall IN : e ∈ rhs, exists e', e' ∈ lhs /\ e' == e) }.
-Next Obligation.
-  split; [intros xs | intros xs ys [xs_ys ys_xs] | intros xs ys zs [xs_ys ys_xs] [ys_zs zs_ys]]; split; i.
-  - exists e. split; auto with *.
-  - exists e. split; auto with *.
-  - find (e1 & H_in & H_eq) by ys_xs. exists e1. split; auto with *.
-  - find (e1 & H_in & H_eq) by xs_ys. exists e1. split; auto with *.
-  - find (e1 & H_in & H_eq) by xs_ys. find (e1' & H_in' & H_eq') by ys_zs. exists e1'. split; auto. transitivity e1; auto with *.
-  - find (e1 & H_in & H_eq) by zs_ys. find (e1' & H_in' & H_eq') by ys_xs. exists e1'. split; auto. transitivity e1; auto with *.
-Qed.
+Context {A : Type} {POSET : isPoset A} {HS_ORD : HsOrd A (POSET := POSET)}.
 
 #[global]
-Instance fin_ensemble_isSetoid1 : isSetoid1 fin_ensemble@{U_fs} :=
-  fin_ensemble_isSetoid.
+Instance fset_corresponds_to_ensemble : Similarity (fset A) (ensemble A) :=
+  Similarity_fset_ensemble eq.
 
-Lemma fin_ensemble_isSetoid1_eq_iff (A : Type@{U_fs}) (xs : fin_ensemble@{U_fs} A) (xs' : fin_ensemble@{U_fs} A)
-  : eqProp (isSetoid := fromSetoid1 fin_ensemble_isSetoid) xs xs' <-> (forall e : A, e ∈ xs <-> e ∈ xs').
+Theorem fset_corresponds_to_ensemble_iff (X : fset A) (X' : ensemble A)
+  : X =~= X' <-> (forall z : A, z ∈ X.(FSet.data) <-> z \in X').
 Proof.
-  ii; ss!.
+  done.
 Qed.
 
-#[global, universes(polymorphic=yes)]
-Instance fin_ensemble_isMonad@{u} : isMonad@{u u} fin_ensemble@{u} :=
-  { pure {A : Type@{u}} (x : A) := (@L.cons A x (@L.nil A))
-  ; bind {A : Type@{u}} {B : Type@{u}} (xs : list A) (k : A -> list B) := (@flat_map A B k xs)
-  }.
+End SIMILARITY.
 
-#[global]
-Instance fin_ensemble_MonadLaws
-  : MonadLaws fin_ensemble (SETOID1 := fin_ensemble_isSetoid1) (MONAD := fin_ensemble_isMonad@{U_fs}).
-Proof.
-  split; i; rewrite fin_ensemble_isSetoid1_eq_iff in *; i; ss!; ss!; exists x0; ss!.
-Qed.
+Section BASICS.
 
-Lemma in_fin_ensemble_bind_intro {A : Type} {B : Type} (xs : fin_ensemble A) (k : A -> fin_ensemble B) (x : A) (y : B)
-  (x_in : L.In x xs)
-  (y_in : L.In y (k x))
-  : L.In y (xs >>= k).
-Proof.
-  cbn [bind fin_ensemble_isMonad]. rewrite L.in_flat_map. eauto.
-Qed.
+Context {A : Type} {POSET : isPoset A} {HS_ORD : HsOrd A (POSET := POSET)}.
 
-Lemma in_fin_ensemble_bind_elim {A : Type} {B : Type} (xs : fin_ensemble A) (k : A -> fin_ensemble B) (y : B)
-  (IN : L.In y (xs >>= k))
-  : exists x, L.In x xs /\ L.In y (k x).
-Proof.
-  cbn [bind fin_ensemble_isMonad] in IN. rewrite L.in_flat_map in IN. exact IN.
-Qed.
-
-Definition mem {A : Type@{U_fs}} `{EQ_DEC : hasEqDec A} (x : A) (xs : fin_ensemble A) : bool :=
-  if in_dec EQ_DEC x xs then true else false.
-
-Theorem mem_spec (A : Type) `(EQ_DEC : hasEqDec A) (x : A) (xs : fin_ensemble A)
-  : forall b, mem x xs = b <-> (if b then x ∈ xs else ~ x ∈ xs).
-Proof.
-  unfold mem; intros [ | ]; revert x; induction xs; intros; simpl; des_ifs; done.
-Qed.
-
-#[global] Hint Rewrite mem_spec : simplication_hints.
-
-Definition add {A : Type@{U_fs}} `{EQ_DEC : hasEqDec A} (x : A) (xs : fin_ensemble A) : fin_ensemble A :=
-  if mem x xs then xs else x :: xs.
-
-Theorem in_add_iff (A : Type) `(EQ_DEC : hasEqDec A) (x : A) (xs : fin_ensemble A)
-  : forall y, y ∈ add x xs <-> (x = y \/ y ∈ xs).
-Proof.
-  i; unfold add, mem; des_ifs; done.
-Qed.
-
-#[global] Hint Rewrite in_add_iff : simplication_hints.
-
-Fixpoint union {A : Type@{U_fs}} `{EQ_DEC : hasEqDec A} (xs : fin_ensemble A) (ys : fin_ensemble A) {struct xs} : fin_ensemble A :=
+Definition insert (x : A) : list A -> list A :=
+  fix go (xs : list A) {struct xs} : list A :=
   match xs with
-  | [] => ys
-  | x :: xs' => union xs' (add x ys)
+  | [] => [x]
+  | y :: ys =>
+    match compare x y with
+    | Lt => x :: y :: ys
+    | Eq => y :: ys
+    | Gt => y :: go ys
+    end
   end.
 
-Theorem in_union_iff (A : Type) `(EQ_DEC : hasEqDec A) (xs : fin_ensemble A) (ys : fin_ensemble A)
-  : forall z, z ∈ union xs ys <-> (z ∈ xs \/ z ∈ ys).
+Lemma in_insert_iff (x : A) (xs : list A)
+  : forall z : A, z ∈ insert x xs <-> (x = z \/ z ∈ xs).
 Proof.
-  revert ys; induction xs as [ | x xs IH]; ii; simpl; s!.
+  induction xs as [ | y ys IH]; intros z; simpl.
   - tauto.
-  - rewrite IH; s!; tauto.
+  - destruct (compare x y) as [ | | ] eqn: H_OBS.
+    + rewrite compare_eq_iff in H_OBS. subst y. simpl. tauto.
+    + simpl. tauto.
+    + simpl. rewrite IH. tauto.
 Qed.
 
-#[global] Hint Rewrite in_union_iff : simplication_hints.
-
-Fixpoint normalize {A : Type@{U_fs}} `{EQ_DEC : hasEqDec A} (xs : fin_ensemble A) {struct xs} : fin_ensemble A :=
-  match xs with
-  | [] => []
-  | x :: xs' => add x (normalize xs')
-  end.
-
-Theorem in_normalize_iff (A : Type) `(EQ_DEC : hasEqDec A) (xs : fin_ensemble A)
-  : forall z, z ∈ normalize xs <-> z ∈ xs.
+Lemma isSorted_insert (x : A) (xs : list A)
+  (xs_isSorted : isSorted compare xs = true)
+  : isSorted compare (insert x xs) = true.
 Proof.
-  induction xs as [ | x xs IH]; simpl; ii; done.
+  revert xs_isSorted. induction xs as [ | y ys IH]; intros xs_isSorted; simpl; trivial.
+  rewrite isSorted_cons_iff in xs_isSorted. destruct xs_isSorted as [y_lt_ys ys_isSorted].
+  destruct (compare x y) as [ | | ] eqn: H_OBS.
+  - rewrite isSorted_cons_iff. split; assumption.
+  - rewrite isSorted_cons_iff. split.
+    + intros z [y_eq_z | z_in_ys]; [congruence | ].
+      exact (compare_Lt_trans x y z H_OBS (y_lt_ys z z_in_ys)).
+    + rewrite isSorted_cons_iff. split; assumption.
+  - rewrite isSorted_cons_iff. split.
+    + intros z z_in. rewrite in_insert_iff in z_in. destruct z_in as [x_eq_z | z_in_ys].
+      * subst z. exact (compare_Gt_flip x y H_OBS).
+      * exact (y_lt_ys z z_in_ys).
+    + exact (IH ys_isSorted).
 Qed.
 
-#[global] Hint Rewrite in_normalize_iff : simplication_hints.
-
-Fixpoint unions {A : Type@{U_fs}} `{EQ_DEC : hasEqDec A} (xss : fin_ensemble (fin_ensemble A)) {struct xss} : fin_ensemble A :=
-  match xss with
-  | [] => []
-  | xs :: xss' => union xs (unions xss')
-  end.
-
-Lemma in_unions_iff (A : Type) `(EQ_DEC : hasEqDec A) (xss : fin_ensemble (fin_ensemble A))
-  : forall z, z ∈ unions xss <-> (exists xs, xs ∈ xss /\ z ∈ xs).
+Lemma length_insert (x : A) (xs : list A)
+  (NOT_IN : ~ x ∈ xs)
+  : length (insert x xs) = S (length xs).
 Proof.
-  induction xss as [ | xs xss IH]; simpl; i; ss!.
-Qed.
-
-#[global] Hint Rewrite in_unions_iff : simplication_hints.
-
-Lemma remove_length_lt {A : Type} `{EQ_DEC : hasEqDec A} (x : A) (xs : list A)
-  (IN : x ∈ xs)
-  : length (remove EQ_DEC x xs) < length xs.
-Proof.
-  revert x IN; induction xs as [ | y ys IH]; simpl; ii.
-  - ss!.
-  - des_ifs.
-    + find ? by remove_length_le; ss!.
-    + des; ss!.
-Qed.
-
-Fixpoint powerset {A : Type@{U_fs}} (xs : fin_ensemble A) : fin_ensemble (fin_ensemble A) :=
-  match xs with
-  | [] => [[]]
-  | x :: xs' =>
-    let ps := powerset xs' in
-    ps ++ map (fun ys => x :: ys) ps
-  end.
-
-Lemma filter_in_powerset {A : Type} (p : A -> bool) (xs : fin_ensemble A)
-  : filter p xs ∈ powerset xs.
-Proof.
-  induction xs as [ | x xs IH]; simpl; des_ifs; ss!.
-Qed.
-
-Lemma powerset_length@{u} {A : Type@{u}} (xs : fin_ensemble A)
-  : length (powerset xs) = pow2 (length xs).
-Proof.
-  induction xs as [ | x xs IH]; simpl.
+  revert NOT_IN. induction xs as [ | y ys IH]; intros NOT_IN; simpl; trivial.
+  destruct (compare x y) as [ | | ] eqn: H_OBS; simpl.
+  - rewrite compare_eq_iff in H_OBS. subst y. contradiction NOT_IN. now left.
   - reflexivity.
-  - rewrite length_app, length_map, IH. f_equal.
-    transitivity (pow2 (length xs)); [exact IH | symmetry; apply Nat.add_0_r].
+  - f_equal. eapply IH. intros z_in. contradiction NOT_IN. now right.
 Qed.
 
-#[universes(polymorphic=yes)]
-Definition product@{u v} {A : Type@{u}} {B : Type@{v}} (xs : list A) (ys : list B) : list (A * B) :=
-  xs >>= fun x => ys >>= fun y => pure (x, y).
-
-Theorem product_iff (A : Type) (B : Type) (xs : fin_ensemble A) (ys : fin_ensemble B)
-  : forall x, forall y, (x, y) ∈ product xs ys <-> (x ∈ xs /\ y ∈ ys).
+Lemma isSorted_fold_right_insert (xs : list A) (ys : list A)
+  (ys_isSorted : isSorted compare ys = true)
+  : isSorted compare (L.fold_right insert ys xs) = true.
 Proof.
-  ii; unfold product; split; intros H_in.
-  - done.
-  - s!. exists (concat (map (fun y => pure (x, y)) ys)). s!. split.
-    + exists x. ss!.
-    + exists [(x, y)]. ss!.
+  induction xs as [ | x xs IH]; simpl; trivial.
+  exact (isSorted_insert x (L.fold_right insert ys xs) IH).
 Qed.
 
-#[global] Hint Rewrite product_iff : simplication_hints.
-
-Lemma in_list_bind_intro {A : Type} {B : Type} (xs : list A) (k : A -> list B) (x : A) (y : B)
-  (x_in : x ∈ xs)
-  (y_in : y ∈ k x)
-  : y ∈ (xs >>= k).
+Lemma in_fold_right_insert_iff (xs : list A) (ys : list A)
+  : forall z : A, z ∈ L.fold_right insert ys xs <-> (z ∈ xs \/ z ∈ ys).
 Proof.
-  rewrite L.list_bind_flat_map. rewrite in_flat_map; eauto.
+  induction xs as [ | x xs IH]; intros z; simpl.
+  - tauto.
+  - rewrite in_insert_iff, IH. tauto.
 Qed.
 
-Lemma in_list_bind_elim {A : Type} {B : Type} (xs : list A) (k : A -> list B) (y : B)
-  (IN : y ∈ (xs >>= k))
-  : exists x, x ∈ xs /\ y ∈ k x.
+Definition empty : fset A :=
+  FSet.mk [] eq_refl.
+
+Definition add (x : A) (X : fset A) : fset A :=
+  FSet.mk (insert x X.(FSet.data)) (isSorted_insert x X.(FSet.data) X.(FSet.data_isSorted)).
+
+Definition fromList (xs : list A) : fset A :=
+  FSet.mk (L.fold_right insert [] xs) (isSorted_fold_right_insert xs [] eq_refl).
+
+Definition union (X : fset A) (X' : fset A) : fset A :=
+  FSet.mk (L.fold_right insert X'.(FSet.data) X.(FSet.data)) (isSorted_fold_right_insert X.(FSet.data) X'.(FSet.data) X'.(FSet.data_isSorted)).
+
+Definition unions (Xs : fset (fset A)) : fset A :=
+  L.fold_right union empty Xs.(FSet.data).
+
+Fixpoint mem' (x : A) (xs : list A) {struct xs} : bool :=
+  match xs with
+  | [] => false
+  | y :: ys =>
+    match compare x y with
+    | Eq => true
+    | _ => mem' x ys
+    end
+  end.
+
+Definition mem (x : A) (X : fset A) : bool :=
+  mem' x X.(FSet.data).
+
+Definition isSubsetOf (X : fset A) (X' : fset A) : Prop :=
+  forall z : A, z ∈ X.(FSet.data) -> z ∈ X'.(FSet.data).
+
+Theorem in_empty_iff
+  : forall z : A, z ∈ empty.(FSet.data) <-> False.
 Proof.
-  induction xs as [ | x xs IH]; ss!.
+  intros z. reflexivity.
 Qed.
 
-Lemma in_list_pure_intro {A : Type} (x : A)
-  : x ∈ pure x.
+Theorem in_add_iff (x : A) (X : fset A)
+  : forall z : A, z ∈ (add x X).(FSet.data) <-> (x = z \/ z ∈ X.(FSet.data)).
 Proof.
-  now simpl; left.
+  exact (in_insert_iff x X.(FSet.data)).
 Qed.
 
-Lemma forallb_false_exists {A : Type} (p : A -> bool) (xs : list A)
-  (FORALL : forallb p xs = false)
-  : exists x, x ∈ xs /\ p x = false.
+Theorem in_fromList_iff (xs : list A)
+  : forall z : A, z ∈ (fromList xs).(FSet.data) <-> z ∈ xs.
 Proof.
-  induction xs as [ | x xs IH]; s!; [congruence | des; ss!].
+  intros z. unfold fromList. simpl. rewrite in_fold_right_insert_iff. simpl. tauto.
 Qed.
 
-Lemma find_some_exists {A : Type} (p : A -> bool) (xs : list A) (x : A)
-  (IN : x ∈ xs)
-  (YES : p x = true)
-  : exists y, find p xs = Some y.
+Lemma length_fromList (xs : list A)
+  (NO_DUP : L.NoDup xs)
+  : length (fromList xs).(FSet.data) = length xs.
 Proof.
-  revert x IN YES; induction xs as [ | x0 xs IH]; ss!; des_ifs; eauto.
+  induction NO_DUP as [ | x xs NOT_IN NO_DUP IH]; trivial.
+  change (length (insert x (fromList xs).(FSet.data)) = S (length xs)).
+  rewrite length_insert.
+  - f_equal. exact IH.
+  - rewrite in_fromList_iff. exact NOT_IN.
 Qed.
 
-Theorem NoDup_exists_injective_length {A : Type} {B : Type} `{B_hasEqDec : hasEqDec B} (xs : list A) (ys : list B) (R : A -> B -> Prop)
-  (xs_NoDup : NoDup xs)
-  (R_total : forall x, x ∈ xs -> (exists y, y ∈ ys /\ R x y))
-  (R_functional : forall x1, forall x2, forall y, x1 ∈ xs -> x2 ∈ xs -> R x1 y -> R x2 y -> x1 = x2)
-  : length xs <= length ys.
+Theorem in_union_iff (X : fset A) (X' : fset A)
+  : forall z : A, z ∈ (union X X').(FSet.data) <-> (z ∈ X.(FSet.data) \/ z ∈ X'.(FSet.data)).
 Proof.
-  revert ys R_total R_functional; induction xs_NoDup as [ | x xs NOT_IN NO_DUP IH]; intros ys TOTAL INJ; simpl; [lia | ].
-  pose proof (TOTAL x (or_introl eq_refl)) as (y & IN_Y & R_XY).
-  enough (LE : length xs <= length (remove B_hasEqDec y ys)).
-  { pose proof (remove_length_lt y ys IN_Y). lia. }
-  eapply IH.
-  - intros x' IN_XS.
-    pose proof (TOTAL x' (or_intror IN_XS)) as (y' & IN_Y' & R_XY').
-    exists y'. split; eauto. rewrite L.in_remove_iff. split; eauto; ii.
-    enough (x' = x) by done!.
-    eapply INJ; ss!.
-  - ii; eapply INJ; ss!.
+  exact (in_fold_right_insert_iff X.(FSet.data) X'.(FSet.data)).
 Qed.
+
+Theorem in_unions_iff (Xs : fset (fset A))
+  : forall z : A, z ∈ (unions Xs).(FSet.data) <-> (exists X : fset A, X ∈ Xs.(FSet.data) /\ z ∈ X.(FSet.data)).
+Proof.
+  unfold unions. generalize Xs.(FSet.data) as Ys. clear Xs.
+  induction Ys as [ | Y Ys IH]; intros z; cbn [L.fold_right].
+  - simpl. split; [tauto | intros (X & [] & _)].
+  - rewrite in_union_iff, IH. simpl. split.
+    + intros [z_in_Y | (X & X_in & z_in_X)].
+      * exists Y. split; [now left | exact z_in_Y].
+      * exists X. split; [now right | exact z_in_X].
+    + intros (X & [Y_eq_X | X_in] & z_in_X).
+      * left. subst X. exact z_in_X.
+      * right. exists X. split; assumption.
+Qed.
+
+Theorem mem_spec (x : A) (X : fset A)
+  : forall b : bool, mem x X = b <-> (if b then x ∈ X.(FSet.data) else ~ x ∈ X.(FSet.data)).
+Proof.
+  assert (claim : mem x X = true <-> x ∈ X.(FSet.data)).
+  { unfold mem. generalize X.(FSet.data) as xs. clear X.
+    induction xs as [ | y ys IH]; simpl.
+    - split; [congruence | tauto].
+    - destruct (compare x y) as [ | | ] eqn: H_OBS.
+      + rewrite compare_eq_iff in H_OBS. subst y. split; [intros _; now left | reflexivity].
+      + rewrite IH. split; [now right | ].
+        intros [y_eq_x | x_in_ys]; trivial.
+        subst y. rewrite compare_refl in H_OBS. discriminate H_OBS.
+      + rewrite IH. split; [now right | ].
+        intros [y_eq_x | x_in_ys]; trivial.
+        subst y. rewrite compare_refl in H_OBS. discriminate H_OBS.
+  }
+  intros [ | ].
+  - exact claim.
+  - split.
+    + intros H_eq x_in. rewrite <- claim in x_in. congruence.
+    + intros NOT_IN. destruct (mem x X) as [ | ] eqn: H_OBS; trivial.
+      contradiction NOT_IN. now rewrite <- claim.
+Qed.
+
+End BASICS.
+
+Section MAP_and_BIND.
+
+Context {A : Type} {POSET_A : isPoset A} {HS_ORD_A : HsOrd A (POSET := POSET_A)}.
+Context {B : Type} {POSET_B : isPoset B} {HS_ORD_B : HsOrd B (POSET := POSET_B)}.
+
+Definition map (f : A -> B) (X : fset A) : fset B :=
+  fromList (L.map f X.(FSet.data)).
+
+Theorem in_map_iff (f : A -> B) (X : fset A)
+  : forall y : B, y ∈ (map f X).(FSet.data) <-> (exists x : A, f x = y /\ x ∈ X.(FSet.data)).
+Proof.
+  intros y. unfold map. rewrite in_fromList_iff. eapply L.in_map_iff.
+Qed.
+
+Definition bind (X : fset A) (k : A -> fset B) : fset B :=
+  L.fold_right (fun x : A => fun Y : fset B => union (k x) Y) empty X.(FSet.data).
+
+Theorem in_bind_iff (X : fset A) (k : A -> fset B)
+  : forall y : B, y ∈ (bind X k).(FSet.data) <-> (exists x : A, x ∈ X.(FSet.data) /\ y ∈ (k x).(FSet.data)).
+Proof.
+  unfold bind. generalize X.(FSet.data) as xs. clear X.
+  induction xs as [ | x xs IH]; intros y; cbn [L.fold_right].
+  - simpl. split; [tauto | intros (? & [] & _)].
+  - rewrite in_union_iff, IH. simpl. split.
+    + intros [y_in_kx | (x' & x'_in & y_in)].
+      * exists x. split; [now left | exact y_in_kx].
+      * exists x'. split; [now right | exact y_in].
+    + intros (x' & [x_eq_x' | x'_in] & y_in).
+      * left. subst x'. exact y_in.
+      * right. exists x'. split; assumption.
+Qed.
+
+End MAP_and_BIND.
+
+Section PRODUCT.
+
+Context {A : Type} {POSET_A : isPoset A} {HS_ORD_A : HsOrd A (POSET := POSET_A)}.
+Context {B : Type} {POSET_B : isPoset B} {HS_ORD_B : HsOrd B (POSET := POSET_B)}.
+
+Definition product (X : fset A) (Y : fset B) : fset (A * B) :=
+  bind X (fun x : A => map (fun y : B => (x, y)) Y).
+
+Theorem product_iff (X : fset A) (Y : fset B)
+  : forall x : A, forall y : B, (x, y) ∈ (product X Y).(FSet.data) <-> (x ∈ X.(FSet.data) /\ y ∈ Y.(FSet.data)).
+Proof.
+  intros x y. unfold product. rewrite in_bind_iff. split.
+  - intros (x' & x'_in_X & xy_in). rewrite in_map_iff in xy_in.
+    destruct xy_in as (y' & H_eq & y'_in_Y). inversion H_eq; subst x' y'.
+    split; assumption.
+  - intros [x_in_X y_in_Y]. exists x. split; trivial.
+    rewrite in_map_iff. exists y. split; trivial.
+Qed.
+
+End PRODUCT.
+
+Section POWERSET.
+
+Context {A : Type} {POSET : isPoset A} {HS_ORD : HsOrd A (POSET := POSET)}.
+
+Lemma isSorted_filter (p : A -> bool) (xs : list A)
+  (xs_isSorted : isSorted compare xs = true)
+  : isSorted compare (L.filter p xs) = true.
+Proof.
+  revert xs_isSorted. induction xs as [ | x xs IH]; intros xs_isSorted; simpl; trivial.
+  rewrite isSorted_cons_iff in xs_isSorted. destruct xs_isSorted as [x_lt_xs xs_isSorted].
+  destruct (p x) as [ | ]; [ | exact (IH xs_isSorted)].
+  rewrite isSorted_cons_iff. split; [ | exact (IH xs_isSorted)].
+  intros z z_in. rewrite L.filter_In in z_in. exact (x_lt_xs z (proj1 z_in)).
+Qed.
+
+Definition filter (p : A -> bool) (X : fset A) : fset A :=
+  FSet.mk (L.filter p X.(FSet.data)) (isSorted_filter p X.(FSet.data) X.(FSet.data_isSorted)).
+
+Theorem in_filter_iff (p : A -> bool) (X : fset A)
+  : forall z : A, z ∈ (filter p X).(FSet.data) <-> (z ∈ X.(FSet.data) /\ p z = true).
+Proof.
+  intros z. exact (L.filter_In p z X.(FSet.data)).
+Qed.
+
+Fixpoint powerset' (xs : list A) {struct xs} : list (fset A) :=
+  match xs with
+  | [] => [empty]
+  | x :: xs' =>
+    let ps := powerset' xs' in
+    ps ++ L.map (add x) ps
+  end.
+
+Definition powerset (X : fset A) : fset (fset A) :=
+  fromList (powerset' X.(FSet.data)).
+
+Lemma in_powerset'_iff (xs : list A)
+  (xs_isSorted : isSorted compare xs = true)
+  : forall Y : fset A, Y ∈ powerset' xs <-> (forall z : A, z ∈ Y.(FSet.data) -> z ∈ xs).
+Proof.
+  revert xs_isSorted. induction xs as [ | x xs IH]; intros xs_isSorted Y.
+  - simpl. split.
+    + intros [empty_eq_Y | []]. subst Y. simpl. tauto.
+    + intros NO_MEM. left. symmetry. rewrite FSet.t_eq_iff.
+      destruct Y as [ys ys_isSorted]. simpl in *.
+      destruct ys as [ | y ys]; trivial.
+      exfalso. exact (NO_MEM y (or_introl eq_refl)).
+  - rewrite isSorted_cons_iff in xs_isSorted. destruct xs_isSorted as [x_lt_xs xs_isSorted].
+    pose proof (IH xs_isSorted) as SPEC. clear IH.
+    cbn [powerset']. rewrite L.in_app_iff, L.in_map_iff. split.
+    + intros [Y_in_ps | (Z & add_eq_Y & Z_in_ps)] z z_in_Y.
+      * right. exact (proj1 (SPEC Y) Y_in_ps z z_in_Y).
+      * subst Y. rewrite in_add_iff in z_in_Y. destruct z_in_Y as [x_eq_z | z_in_Z].
+        { now left. }
+        { right. exact (proj1 (SPEC Z) Z_in_ps z z_in_Z). }
+    + intros Y_sub. destruct (mem x Y) as [ | ] eqn: H_mem.
+      * right. rewrite mem_spec in H_mem.
+        exists (filter (fun z : A => match compare x z with Eq => false | _ => true end) Y). split.
+        { rewrite fset_eq_spec. intros w. rewrite in_add_iff, in_filter_iff. split.
+          - intros [x_eq_w | [w_in _]]; [subst w; exact H_mem | exact w_in].
+          - intros w_in_Y. cbv beta. destruct (compare x w) as [ | | ] eqn: H_OBS.
+            + left. exact (proj1 (compare_eq_iff x w) H_OBS).
+            + right. split; [exact w_in_Y | reflexivity].
+            + right. split; [exact w_in_Y | reflexivity].
+        }
+        { rewrite SPEC. intros z z_in. rewrite in_filter_iff in z_in.
+          destruct z_in as [z_in_Y H_p]. cbv beta in H_p.
+          destruct (Y_sub z z_in_Y) as [x_eq_z | z_in_xs]; trivial.
+          subst z. rewrite compare_refl in H_p. discriminate H_p.
+        }
+      * left. rewrite SPEC. intros z z_in_Y.
+        destruct (Y_sub z z_in_Y) as [x_eq_z | z_in_xs]; trivial.
+        subst z. exfalso. rewrite mem_spec in H_mem. contradiction (H_mem z_in_Y).
+Qed.
+
+Theorem in_powerset_iff (X : fset A)
+  : forall Y : fset A, Y ∈ (powerset X).(FSet.data) <-> isSubsetOf Y X.
+Proof.
+  intros Y. unfold powerset. rewrite in_fromList_iff.
+  exact (in_powerset'_iff X.(FSet.data) X.(FSet.data_isSorted) Y).
+Qed.
+
+Theorem filter_in_powerset (p : A -> bool) (X : fset A)
+  : filter p X ∈ (powerset X).(FSet.data).
+Proof.
+  rewrite in_powerset_iff. intros z z_in.
+  rewrite in_filter_iff in z_in. exact (proj1 z_in).
+Qed.
+
+Lemma NoDup_powerset' (xs : list A)
+  (xs_isSorted : isSorted compare xs = true)
+  : L.NoDup (powerset' xs).
+Proof.
+  revert xs_isSorted. induction xs as [ | x xs IH]; intros xs_isSorted.
+  - simpl. econstructor; [intros [] | econstructor].
+  - rewrite isSorted_cons_iff in xs_isSorted. destruct xs_isSorted as [x_lt_xs xs_isSorted].
+    pose proof (IH xs_isSorted) as NO_DUP. clear IH.
+    pose proof (in_powerset'_iff xs xs_isSorted) as SPEC.
+    assert (x_not_in_xs : ~ x ∈ xs).
+    { intros x_in. pose proof (x_lt_xs x x_in) as LT.
+      rewrite compare_refl in LT. discriminate LT.
+    }
+    assert (claim : forall Y : fset A, Y ∈ powerset' xs -> ~ x ∈ Y.(FSet.data)).
+    { intros Y Y_in x_in_Y. contradiction x_not_in_xs. exact (proj1 (SPEC Y) Y_in x x_in_Y). }
+    cbn [powerset']. eapply L.NoDup_app; trivial.
+    + eapply NoDup_map_inj; trivial. intros Y Z Y_in Z_in H_eq.
+      rewrite fset_eq_spec. intros w. rewrite fset_eq_spec in H_eq.
+      specialize (H_eq w). rewrite !in_add_iff in H_eq.
+      destruct (compare x w) as [ | | ] eqn: H_OBS.
+      * rewrite compare_eq_iff in H_OBS. subst w. split.
+        { intros w_in. contradiction (claim Y Y_in w_in). }
+        { intros w_in. contradiction (claim Z Z_in w_in). }
+      * split.
+        { intros w_in. destruct (proj1 H_eq (or_intror w_in)) as [x_eq_w | H]; trivial.
+          subst w. rewrite compare_refl in H_OBS. discriminate H_OBS.
+        }
+        { intros w_in. destruct (proj2 H_eq (or_intror w_in)) as [x_eq_w | H]; trivial.
+          subst w. rewrite compare_refl in H_OBS. discriminate H_OBS.
+        }
+      * split.
+        { intros w_in. destruct (proj1 H_eq (or_intror w_in)) as [x_eq_w | H]; trivial.
+          subst w. rewrite compare_refl in H_OBS. discriminate H_OBS.
+        }
+        { intros w_in. destruct (proj2 H_eq (or_intror w_in)) as [x_eq_w | H]; trivial.
+          subst w. rewrite compare_refl in H_OBS. discriminate H_OBS.
+        }
+    + intros Y Y_in Y_in'. rewrite L.in_map_iff in Y_in'.
+      destruct Y_in' as (Z & add_eq_Y & Z_in). contradiction (claim Y Y_in).
+      rewrite <- add_eq_Y. rewrite in_add_iff. now left.
+Qed.
+
+Lemma length_powerset' (xs : list A)
+  : length (powerset' xs) = pow2 (length xs).
+Proof.
+  induction xs as [ | x xs IH]; trivial.
+  cbn [powerset' length pow2]. rewrite length_app, length_map, IH. lia.
+Qed.
+
+Theorem powerset_length (X : fset A)
+  : length (powerset X).(FSet.data) = pow2 (length X.(FSet.data)).
+Proof.
+  unfold powerset. rewrite length_fromList.
+  - exact (length_powerset' X.(FSet.data)).
+  - exact (NoDup_powerset' X.(FSet.data) X.(FSet.data_isSorted)).
+Qed.
+
+End POWERSET.
+
+#[global] Hint Rewrite @in_empty_iff @in_add_iff @in_fromList_iff @in_union_iff @in_unions_iff @in_filter_iff @in_map_iff @in_bind_iff @product_iff @in_powerset_iff @mem_spec : simplication_hints.
 
 End FS.
