theories/Prelude/X.v
@@ -12,7 +12,7 @@ Tactic Notation "rewrite*" uconstr( t ) "by" ident ( H_EQ ) :=
 Tactic Notation "find" simple_intropattern( p ) "by" uconstr( H ) :=
   unshelve hexploit H; [eauto .. | intros p].
 
-Tactic Notation "obtain" simple_intropattern( p ) "by" uconstr( H ) :=
+Tactic Notation "find*" simple_intropattern( p ) "by" uconstr( H ) :=
   hexploit H; [eauto .. | intros p].
 
 Ltac done :=
@@ -108,3 +108,44 @@ Instance falsum_dec
 Proof.
   right. intros H. exact H.
 Defined.
+
+Lemma remove_length_lt {A : Type} `{EQ_DEC : hasEqDec A} (x : A) (xs : list A)
+  (IN : L.In x xs)
+  : length (remove EQ_DEC x xs) < length xs.
+Proof.
+  revert x IN; induction xs as [ | y ys IH]; simpl; ii.
+  - ss!.
+  - des_ifs.
+    + find ? by remove_length_le; ss!.
+    + des; ss!.
+Qed.
+
+Theorem NoDup_exists_injective_length {A : Type} {B : Type} `{B_hasEqDec : hasEqDec B} (xs : list A) (ys : list B) (R : A -> B -> Prop)
+  (xs_NoDup : NoDup xs)
+  (R_total : forall x, L.In x xs -> (exists y, L.In y ys /\ R x y))
+  (R_functional : forall x1, forall x2, forall y, L.In x1 xs -> L.In x2 xs -> R x1 y -> R x2 y -> x1 = x2)
+  : length xs <= length ys.
+Proof.
+  revert ys R_total R_functional; induction xs_NoDup as [ | x xs NOT_IN NO_DUP IH]; intros ys TOTAL INJ; simpl; [lia | ].
+  pose proof (TOTAL x (or_introl eq_refl)) as (y & IN_Y & R_XY).
+  enough (LE : length xs <= length (remove B_hasEqDec y ys)).
+  { pose proof (remove_length_lt y ys IN_Y). lia. }
+  eapply IH.
+  - intros x' IN_XS.
+    pose proof (TOTAL x' (or_intror IN_XS)) as (y' & IN_Y' & R_XY').
+    exists y'. split; eauto. rewrite L.in_remove_iff. split; eauto; ii.
+    enough (x' = x) by done!.
+    eapply INJ; ss!.
+  - ii; eapply INJ; ss!.
+Qed.
+
+Lemma NoDup_map_inj {X : Type} {Y : Type} (f : X -> Y) (l : list X)
+  (NO_DUP : L.NoDup l)
+  (INJ : forall a : X, forall b : X, L.In a l -> L.In b l -> f a = f b -> a = b)
+  : L.NoDup (L.map f l).
+Proof.
+  revert INJ. induction NO_DUP as [ | a l NOT_IN NO_DUP IH]; intros ?; simpl; econs.
+  - intros H_in. rewrite L.in_map_iff in H_in. destruct H_in as (b & f_eq & b_in).
+    contradiction NOT_IN. erewrite INJ with (a := a) (b := b); simpl; eauto with *.
+  - eapply IH. intros a1 b1 a1_in b1_in H_eq.  exact (INJ a1 b1 (or_intror a1_in) (or_intror b1_in) H_eq).
+Qed.
